\documentclass[problem]{mcs}

\begin{pcomments}
  \pcomment{FP_recurrence_strong_induction}
  \pcomment{from F10, practiceprobems}
  \pcomment{edited ARM 5/16/15}
\end{pcomments}

\pkeywords{
  strong_induction
  induction
  congruence
  linear_recurrence
  recurrence
}

\begin{problem}
We define the sequence of numbers
\[
a_n = \begin{cases}
  1,   &  \text{for $n \leq 3$,}\\
  a_{n-1} + a_{n-2} + a_{n-3}+ a_{n-4},
      &  \text{for $n > 3$.}
 \end{cases}
\]

Use \emph{strong induction} to prove that $\text{remainder}(a_n,3) =
1$ for all $n\geq 0$.

\begin{solution}
We use the fact that $\rem{m}{3} = 1$ iff $m \equiv 1 \pmod 3$.
Letting
\[
P(n)\eqdef\quad a_n \equiv 1 \pmod 3,
\]
we need only show by strong induction that $P(n)$ is true for all $n$.

\inductioncase{Base case} ($n\leq 3$): $a_n \eqdef 1$, so $a_n \equiv
1 \pmod 3$.

\inductioncase{Inductive step}: For $n > 3$, assume $P(k)$ for $0\leq k < n$ 
in order to prove $P(n)$.

In particular, we may assume that $a_k \equiv 1 \pmod 3$ for $k =
n-4,n-3,n-2,n-1$.  But $P(n)$ is equivalent to $a_{n-4} + a_{n-3} +
a_{n-2} + a_{n-1} = 1 \pmod 3$, so $P(n)$ is true because
\[
a_n = a_{n-4} + a_{n-3} + a_{n-2} + a_{n-1} \equiv (1+1+1+1) = 1 \pmod 3,
\]
\end{solution}

\end{problem}

\endinput
