\documentclass[handout]{mcs}

\begin{document}

\renewcommand{\reading}{
  Final
}

\problemset{F}

%%%%%%%%%%%%%%%%%%%%%%%%%%%%%%%%%%%%%%%%%%%%%%%%%%%%%%%%%%%%%%%%%%%%%
% Problems start here
%%%%%%%%%%%%%%%%%%%%%%%%%%%%%%%%%%%%%%%%%%%%%%%%%%%%%%%%%%%%%%%%%%%%%

\pinput{FP_logic_of_leq}

\pinput{FP_counting_given_answers}

\pinput{FP_structural_induction_arithmetic_expressions}

\pinput{FP_paths_inclusion_exclusion}

\begin{problem}
A Lucas number is defined as follows:
\begin{equation}
  L_n :=
  \begin{cases}
    2               & \text{if } n = 0; \\
    1               & \text{if } n = 1; \\
    L_{n-1}+L_{n-2} & \text{if } n > 1. \\
   \end{cases}
\end{equation}

Prove by induction that for all $n \geq 2$,

$$ L_n L_{n-2} - L_{n-1}^2 = 5 (-1)^n$$.

\begin{solution}

Base case: $n=2$ ($L_2 = 3$):

$$L_2 L_0 - L_1^2 = 3 \cdot 2 - 1^2 = 5$$

Let's prove by induction. Say that for every $i \leq n$: $L_i L_{i-2} - L_{i-1}^2 = 5 \cdot (-1)^n$, then:

$$L_{n+1} L_{n-1} - L_n^2$$

$$= (L_n+L_{n-1}) L_{n-1} - L_n^2 \mbox{ (definition of Lucas number)}$$

$$ = L_n L_{n-1} + L_{n-1}^2 -L_n^2 \mbox{ (distributive law)}$$

$$ = L_n L_{n-1} - L_n^2 +L_{n-1}^2 \mbox{ (reordering terms)}$$

$$ = L_n(L_{n-1} -L_n) + L_{n-1}^2 $$

$$ = -L_n L_{n-2} + L_{n-1}^2  \mbox{ definition of Lucas number}$$

$$ = - 5 (-1)^n = 5  (-1)^{n+1}$$

\end{solution}

\end{problem}

%%%%%%%%%%%%%%%%%%%%%%%%%%%%%%%%%%%%%%%%%%%%%%%%%%%%%%%%%%%%%%%%%%%%%
% Problems end here
%%%%%%%%%%%%%%%%%%%%%%%%%%%%%%%%%%%%%%%%%%%%%%%%%%%%%%%%%%%%%%%%%%%%%

\end{document}
