\documentclass[problem]{mcs}

\begin{pcomments}
  \pcomment{from: S09.cp9m}
  \pcomment{from: S05.rec10}
\end{pcomments}

\pkeywords{
  series
  closed_form
}

%%%%%%%%%%%%%%%%%%%%%%%%%%%%%%%%%%%%%%%%%%%%%%%%%%%%%%%%%%%%%%%%%%%%%
% Problem starts here
%%%%%%%%%%%%%%%%%%%%%%%%%%%%%%%%%%%%%%%%%%%%%%%%%%%%%%%%%%%%%%%%%%%%%

\begin{problem}
You've seen this neat trick for evaluating a geometric sum:
%
\begin{align*}
S & = 1 + z + z^2 + \ldots + z^n \\
zS & = z + z^2 + \ldots + z^n + z^{n+1} \\
S - z S & = 1 - z^{n+1} \\
S & = \frac{1-z^{n+1}}{1 - z}
\end{align*}

Use the same approach to find a closed-form expression for this sum:
%
\begin{align*}
T & = 1 z + 2 z^2 + 3 z^3 + \ldots + n z^n
\end{align*}

\solution{
\begin{align*}
z T & = 1 z^2 + 2 z^3 + 3 z^4 + \ldots + n z^{n+1} \\
T - zT & = z + z^2 + z^3 + \ldots + z^n - n z^{n+1} \\
       & = \frac{1 - z^{n+1}}{1 - z} - 1 - n z^{n+1} \\
T & = \frac{1 - z^{n+1}}{(1 - z)^2} - \frac{1 + n z^{n+1}}{1 - z}
\end{align*}
}

\end{problem}

%%%%%%%%%%%%%%%%%%%%%%%%%%%%%%%%%%%%%%%%%%%%%%%%%%%%%%%%%%%%%%%%%%%%%
% Problem ends here
%%%%%%%%%%%%%%%%%%%%%%%%%%%%%%%%%%%%%%%%%%%%%%%%%%%%%%%%%%%%%%%%%%%%%
