\documentclass[problem]{mcs}

%%%%%%%%%%%%%%%%%%%%%%%%%%%%%%%%%%%%%%%%%%%%%%%%%%%%%%%%%%%%%%%%%%%%%
% Problem starts here
%%%%%%%%%%%%%%%%%%%%%%%%%%%%%%%%%%%%%%%%%%%%%%%%%%%%%%%%%%%%%%%%%%%%%

% S09, S06

\begin{problem}

\bparts

The following properties of equivalence mod $n$ follow directly from its
definition and simple properties of divisibility.  See if you can prove
them without looking up the proofs in the notes.

\ppart\label{multc} If $a \equiv b \pmod{n}$, then $a c \equiv b c
\pmod{n}$.

\solution{The condition $a \equiv b \pmod{n}$ is equivalent to the
assertion $n \divides (a - b)$.  This implies that $n \divides (a - b)c$,
and so $n \divides (ac - bc)$.  This is equivalent to $ac \equiv bc
\pmod{n}$.}

\ppart\label{transitive} If $a \equiv b \pmod{n}$ and $b \equiv c
\pmod{n}$, then $a \equiv c \pmod{n}$.

\solution{Assume $a \equiv b \pmod{n}$ and $b \equiv c \pmod{n}$, that is,
$n \divides (a - b)$ and $n \divides (b - c)$.  Then $n \divides (a - b) +
(b - c) = (a-c)$, so $a \equiv c \pmod{n}$.}

\ppart If $a \equiv b \pmod{n}$ and $c \equiv d \pmod{n}$, then $a c
\equiv b d \pmod{n}$.

\solution{$a \equiv b \pmod{n}$ implies $ac \equiv bc \pmod{n}$ by
part~\eqref{multc}; likewise, $c \equiv d \pmod{n}$ implies $bc \equiv bd
\pmod{n}$.  So $a c \equiv b d \pmod{n}$ by part~\eqref{transitive}.}

\ppart $\rem{a}{n} \equiv a \pmod{n}$.

\solution{The remainder $\rem{a}{n}$ is equal to $a - qn$ for some integer
$q$.  However, for every integer $q$:
\begin{align*}
n \divides qn &  \iff  n \divides ((a - qn) - a) \\
              &  \implies  n \divides (\rem{a}{n} - a)\\
              & \iff  \rem{a}{n} \equiv a \pmod{n}.
\end{align*}}
\eparts

\end{problem}

%%%%%%%%%%%%%%%%%%%%%%%%%%%%%%%%%%%%%%%%%%%%%%%%%%%%%%%%%%%%%%%%%%%%%
% Problem ends here
%%%%%%%%%%%%%%%%%%%%%%%%%%%%%%%%%%%%%%%%%%%%%%%%%%%%%%%%%%%%%%%%%%%%%

\endinput
