\documentclass[problem]{mcs}

\begin{pcomments}
  \pcomment{FP_lucas_induction}
  \pcomment{Giuliano, May 2012}}
\end{pcomments}

\pkeywords{
  induction
  strong_induction
}

%%%%%%%%%%%%%%%%%%%%%%%%%%%%%%%%%%%%%%%%%%%%%%%%%%%%%%%%%%%%%%%%%%%%%
% Problem starts here
%%%%%%%%%%%%%%%%%%%%%%%%%%%%%%%%%%%%%%%%%%%%%%%%%%%%%%%%%%%%%%%%%%%%%

\begin{problem}[Induction]

A Lucas number is defined as follows:
\begin{equation}
  L_n \eqdef
  \begin{cases}
    2               & \text{if } n = 0; \\
    1               & \text{if } n = 1; \\
    L_{n-1}+L_{n-2} & \text{if } n > 1. \\
   \end{cases}
\end{equation}

Prove by induction that for all $n \geq 2$,
\[
L_n L_{n-2} - L_{n-1}^2 = 5 (-1)^n.
\]

\begin{solution}

Base case: $n=2$ ($L_2 = 3$):

$$L_2 L_0 - L_1^2 = 3 \cdot 2 - 1^2 = 5$$

Let's prove by induction. Say that for every $i \leq n$: $L_i L_{i-2} - L_{i-1}^2 = 5 \cdot (-1)^n$, then:
\begin{align*}
L_{n+1} L_{n-1} - L_n^2
 &= (L_n+L_{n-1}) L_{n-1} - L_n^2  & \mbox{ (definition of Lucas number)}\\
 & = L_n L_{n-1} + L_{n-1}^2 -L_n^2 & \mbox{ (distributive law)}\\
 & = L_n L_{n-1} - L_n^2 +L_{n-1}^2  & \mbox{ (reordering terms)}\\
 & = L_n(L_{n-1} -L_n) + L_{n-1}^2\\
 & = -L_n L_{n-2} + L_{n-1}^2  & \mbox{ definition of Lucas number}$$
 & = - 5 (-1)^n = 5  (-1)^{n+1}
\end{align*}

\end{solution}

\end{problem}


%%%%%%%%%%%%%%%%%%%%%%%%%%%%%%%%%%%%%%%%%%%%%%%%%%%%%%%%%%%%%%%%%%%%%
% Problem ends here
%%%%%%%%%%%%%%%%%%%%%%%%%%%%%%%%%%%%%%%%%%%%%%%%%%%%%%%%%%%%%%%%%%%%%

\endinput
