\documentclass[problem]{mcs}

\begin{pcomments}
  \pcomment{MQ_sum_of_cubes}
  \pcomment{by Giu, Peter 2/16/12}
  \pcomment{reformatted by ARM 3/6/13}
\end{pcomments}

\pkeywords{
  induction
}


%%%%%%%%%%%%%%%%%%%%%%%%%%%%%%%%%%%%%%%%%%%%%%%%%%%%%%%%%%%%%%%%%%%%%
% Problem starts here
%%%%%%%%%%%%%%%%%%%%%%%%%%%%%%%%%%%%%%%%%%%%%%%%%%%%%%%%%%%%%%%%%%%%%


\begin{problem}
Prove by induction:
\[
0^3 + 1^3 + 2^3 + \cdots + n^3  = \paren{\frac{n(n+1)}{2}}^{2}, \forall n \geq 0.
\]
using the equation itself as the induction hypothesis $P(n)$.

\bparts

\ppart Prove the \inductioncase{base case} $(n=0)$.

\begin{solution}
  \[
   0^3 = = 0 = \paren{\frac{0\cdot 1}{2}}^2.
  \]
Therefore, $P(0)$ is true.
\end{solution}

\examspace[2in]

\ppart Now prove the \inductioncase{inductive step}.

\begin{solution}
\begin{align*}
\sum_{i=0}^{n+1} i^3
 & = \sum_{i=0}^{n} i^3 + (n+1)^3\\
 & = \paren{\frac{n(n+1)}{2}}^{2} + (n+1)^3 & \text{(by induction hypothesis $P(n)$)}\\
 & = (n+1)^2 \paren{\paren{\frac{n}{2}}^{2} + (n+1)}\\
 & = (n+1)^2 \paren{\frac{n^2}{4} + \frac{4n+4}{4}}\\
 & = (n+1)^2 \frac{n^2 + 4n + 4}{4}\\
 & = (n+1)^2 \frac{(n+2)^2}{4}\\
 & = \paren{\frac{(n+1)(n+2)}{2}}^{2}.
\end{align*}
Thus we have proved $P(n+1)$, completing the induction step.

We conclude by induction that $P(n)$ holds for all $n \in \nngint$.
\end{solution}

\eparts

\end{problem}

%%%%%%%%%%%%%%%%%%%%%%%%%%%%%%%%%%%%%%%%%%%%%%%%%%%%%%%%%%%%%%%%%%%%%
% Problem ends here
%%%%%%%%%%%%%%%%%%%%%%%%%%%%%%%%%%%%%%%%%%%%%%%%%%%%%%%%%%%%%%%%%%%%%

\endinput
