\documentclass[problem]{mcs}

\begin{pcomments}
  \pcomment{from: S09.ps8}
  \pcomment{practice with sum formulas}
  \pcomment{double sum tricks not used in class}
\end{pcomments}

\pkeywords{
  geometric
  arithmetic
  sum
  series
  closed_form
}

%%%%%%%%%%%%%%%%%%%%%%%%%%%%%%%%%%%%%%%%%%%%%%%%%%%%%%%%%%%%%%%%%%%%%
% Problem starts here
%%%%%%%%%%%%%%%%%%%%%%%%%%%%%%%%%%%%%%%%%%%%%%%%%%%%%%%%%%%%%%%%%%%%%

\begin{problem}
Find closed-form expressions for the following sums.

\bparts

\ppart

\[
\sum_{i=0}^n \frac{9^i - 7^i}{11^i}
\]

\begin{solution}
Split the expression into two \idx{geometric series} and then
apply the formula for the sum of a geometric series.
%
\begin{align*}
\sum_{i=0}^n \frac{9^i - 7^i}{11^i}
    & = \sum_{i=0}^n \left(\frac{9}{11}\right)^i -
        \sum_{i=0}^n \left(\frac{7}{11}\right)^i \\
    & = \frac{1 - \left(\frac{9}{11}\right)^{n+1}}{1 - \frac{9}{11}}
          - \frac{1 - \left(\frac{7}{11}\right)^{n+1}}{1 - \frac{7}{11}} \\
    & = - \frac{11}{2} \cdot \left(\frac{9}{11}\right)^{n+1}
        + \frac{11}{4} \cdot \left(\frac{7}{11}\right)^{n+1}
        + \frac{11}{4}
\end{align*}

\end{solution}

\ppart\label{sum3m3n}

\[
\sum_{i=0}^n \sum_{j=0}^m 3^{i+j}
\]

\begin{solution}
\begin{align*}
\sum_{i=0}^n \sum_{j=0}^m 3^{i+j}
    & = \sum_{i=0}^n \left(3^i \cdot \sum_{j=0}^m 3^j\right) \\
    & = \sum_{i=0}^n 3^i \frac{3^{m+1} - 1}{2} \\
    & = \frac{3^{m+1} - 1}{2} \sum_{i=0}^n 3^i\\
    & = \frac{3^{m+1} - 1}{2} \cdot \frac{3^{n+1} - 1}{2}
%    & = \frac{\paren{3^{m+1} - 1}\paren{3^{n+1} - 1}}{4}
%    & = \left(\sum_{j=0}^m 3^j\right) \cdot \left(\sum_{i=0}^n 3^i\right)\\
\end{align*}

\end{solution}

\ppart
\[
\sum_{j=1}^n \sum_{i=0}^{\infty} j^{5/3} \cdot \paren{1 - \frac{1}{2 j^{1/3}}}^i
\]

\begin{solution}
This fearsome-looking sum is a paper tiger: as in
part~\eqref{sum3m3n}, we just apply the formula for the inner sum---a
geometric series---which allows the outer sum to be simplified into a
sum of squares, which has a closed form\inbook{ given by
  equation~(\bref{eqn:G27})}.
%
\begin{align*}
\sum_{j=1}^n \sum_{i=0}^{\infty} j^{5/3} \cdot \paren{1 - \frac{1}{2 j^{1/3}}}^i
    & = \sum_{j=1}^n j^{5/3} \cdot \frac{1}{1 - \paren{1 - \frac{1}{2 j^{1/3}}}} \\
    & = \sum_{j=1}^n 2j^2 \\
    & = \frac{2n (n+\frac{1}{2})(n+1)}{3}
\end{align*}

\end{solution}

\eparts
\end{problem}

%%%%%%%%%%%%%%%%%%%%%%%%%%%%%%%%%%%%%%%%%%%%%%%%%%%%%%%%%%%%%%%%%%%%%
% Problem ends here
%%%%%%%%%%%%%%%%%%%%%%%%%%%%%%%%%%%%%%%%%%%%%%%%%%%%%%%%%%%%%%%%%%%%%

\endinput
