\documentclass[problem]{mcs}

\begin{pcomments}
  \pcomment{PS_string_cancellation}
  \pcomment{needed in CP_string_reversal}
  \pcomment{by ARM 3/13/16}
  \pcomment{ARM: pedantic, cut from book, 3/2/17}
\end{pcomments}

\pkeywords{
  string
  structural_induction
  induction
  concatenation
  associativity
  length
}

%%%%%%%%%%%%%%%%%%%%%%%%%%%%%%%%%%%%%%%%%%%%%%%%%%%%%%%%%%%%%%%%%%%%%
% Problem starts here
%%%%%%%%%%%%%%%%%%%%%%%%%%%%%%%%%%%%%%%%%%%%%%%%%%%%%%%%%%%%%%%%%%%%%

\begin{problem}
Prove that if $rs=tu$ for $r,s,t,u \in \strings{A}$, and $\lnth{r}= \lnth{t}$, 
then $r = t$ and $s = u$.

\begin{solution}
\TBA{induction on length of $r$.}  Uses defining property of pairing:
$\ang{x,y} = \ang{z,w}$ implies $x =z$ and $y=w$ for all objects
$x,y,z,w$.
\end{solution}

\end{problem}

%%%%%%%%%%%%%%%%%%%%%%%%%%%%%%%%%%%%%%%%%%%%%%%%%%%%%%%%%%%%%%%%%%%%%
% Problem ends here
%%%%%%%%%%%%%%%%%%%%%%%%%%%%%%%%%%%%%%%%%%%%%%%%%%%%%%%%%%%%%%%%%%%%%

\endinput
