\documentclass[problem]{mcs}

\begin{pcomments}
  \pcomment{from: S06.ps1}
\end{pcomments}

\pkeywords{
  validity
}

%%%%%%%%%%%%%%%%%%%%%%%%%%%%%%%%%%%%%%%%%%%%%%%%%%%%%%%%%%%%%%%%%%%%%
% Problem starts here
%%%%%%%%%%%%%%%%%%%%%%%%%%%%%%%%%%%%%%%%%%%%%%%%%%%%%%%%%%%%%%%%%%%%%

\begin{problem}  Prove that
\[  %\begin{equation}\label{v}
[\forall x.\; \neg P(x)] \implies \neg \exists z.\; P(z).
\]  %\end{equation}
is valid.  (Use the validity proof from the subsection on Validity in
the Course Notes, namely section 5.1.5, as guides to writing your proof.)

\solution{
\begin{proof}
Assume
\begin{equation}\label{eq:1}
\forall x.\; \neg P(x).
\end{equation}

Now we prove by contradiction that $ \neg \exists z.\; P(z)$ holds.
Namely, we assume $\exists z.\; P(z)$ and reach a contradiction.

So suppose $\exists z.\; P(z)$ holds.  So there is an element, $c$,
such that $P(c)$.  But from~\eqref{eq:1}, we know that $\neg P(c)$
holds, contradicting the fact that $P(c)$ holds.  Hence, the
assumption $\exists z.\; P(z)$ must be false, that is, $\neg \exists
z.\; P(z)$ is true.
\end{proof}}

\end{problem}

%%%%%%%%%%%%%%%%%%%%%%%%%%%%%%%%%%%%%%%%%%%%%%%%%%%%%%%%%%%%%%%%%%%%%
% Problem ends here
%%%%%%%%%%%%%%%%%%%%%%%%%%%%%%%%%%%%%%%%%%%%%%%%%%%%%%%%%%%%%%%%%%%%%