\documentclass[problem]{mcs}

\begin{pcomments}
  \pcomment{TP_basic_set_formulas}
  \pcomment{actually subsumes FP_basic_set_formulas}
  \pcomment{ARM 2/17/13}
\end{pcomments}

\pkeywords{
  logic
  sets
  set_theory
  predicate
  formula
  subset
  power_set
  union
}

\begin{problem}
\inhandout{A \emph{formula of set theory} is a predicate formula that
  only uses the predicate ``$x \in y$.''  The domain of discourse is
  the collection of sets, and ``$x \in y$'' is interpreted to mean the
  set $x$ is one of the elements in the set $y$.

For example, since $x$ and $y$ are the same set iff they have the same
members, here's how we can express equality of $x$ and $y$ with a
formula of set theory:
\[
(x = y) \eqdef\ \forall z.\, (z \in x\ \QIFF\ z \in y).
\]
}

Express each of the following assertions about sets by a formula of
set theory.\inbook{\footnote{See Section~\bref{ZFC_sec}.}}
Expressions may use abbreviations introduced earlier (so it is now
legal to use ``$=$'' because we just defined it).

\bparts

\ppart $x = \emptyset$.

\begin{solution}
$\forall z.\, \QNOT(z\in x)$.
\end{solution}

\ppart $x = \set{y,z}$.

\begin{solution}
$\forall w.\, w \in x \QIFF (w=y \QOR\ w = z)$.
\end{solution}

\ppart $x \subseteq y$.  ($x$ is a subset of $y$ that might equal $y$.)

\begin{solution}
$\forall z.\, z \in x\ \QIMPLIES\ z \in y$.
\end{solution}

\eparts 

Now we can explain how to express ``$x$ is a proper
  subset of $y$'' as a set theory formula using
things we already know how to express.  Namely, letting
``$x \neq y$'' abbreviate $\QNOT(x = y)$, the expression
\[
(x \subseteq y\ \QAND\ x \neq y),
\]
describes a formula of set theory that means $x \subset y$.

From here on, feel free to use any previously expressed property in
describing formulas for the following:

\bparts
\ppart $x = y \union z$.

\begin{solution}
$\forall w.\, w \in x \QIFF (w \in y\ \QOR\ w \in z)$.
\end{solution}

\ppart $x = y - z$.

\begin{solution}
$\forall w.\, w \in x\ \QIFF\  (w \in y\ \QAND\ \QNOT(w \in z))$.
\end{solution}

\begin{staffnotes}
Now other ways to express $x \subset y$ are
\[
\exists z.\, (y = x \union z\ \QAND\ z \neq \emptyset).
\]
and
\[
(x - y) = \emptyset.
\]
\end{staffnotes}

\ppart $x = \power(y)$.

\begin{solution}
$\forall z.\, z \in x \QIFF z \subseteq y$.
\end{solution}

\ppart $x = \lgunion_{z \in y} z$.

This means that $y$ is supposed to be a collection of sets, and $x$ is
the union of all of them.  A more concise notation for ``$\lgunion_{z \in
  y} z$' is simply ``$\lgunion y$.''

\begin{solution}
$\forall w.\, w \in x \QIFF \exists z.\, (z \in y\ \QAND\ w \in z)$.
\end{solution}

\eparts

\end{problem}

\endinput
